lean/LoVe/LoVe09_OperationalSemantics_HomeworkSheet.lean
@@ -33,11 +33,48 @@ def Envir : Type :=
 semantics for arithmetic expressions. The predicate `BigStep` (`⟹`) relates
 an arithmetic expression, an environment, and the value to which the expression
 evaluates in the given environment: -/
-
+#print AExp
 inductive BigStep : AExp × Envir → ℤ → Prop
   | num (i env) : BigStep (AExp.num i, env) i
-
+  | var (x env) : BigStep (AExp.var x, env) (env x)
+  | add (a1 a2 v1 v2 env) (ha1: BigStep (a1,env) v1) (ha2: BigStep (a2,env) v2): BigStep (AExp.add a1 a2, env) (v1+v2)
+  | sub (a1 a2 v1 v2 env) (ha1: BigStep (a1,env) v1) (ha2: BigStep (a2,env) v2): BigStep (AExp.sub a1 a2, env) (v1-v2)
+  | mul (a1 a2 v1 v2 env) (ha1: BigStep (a1,env) v1) (ha2: BigStep (a2,env) v2): BigStep (AExp.mul a1 a2, env) (v1*v2)
+  | div (a1 a2 v1 v2 env) (ha1: BigStep (a1,env) v1) (ha2: BigStep (a2,env) v2): BigStep (AExp.div a1 a2, env) (v1/v2)
 infix:60 " ⟹ " => BigStep
+
+@[simp]
+theorem bla (a env i): BigStep (a,env) i ↔ i = (eval env a) := by
+  apply Iff.intro
+  · intro h
+    induction a generalizing i with
+    | num _ => cases h; simp [eval]
+    | var _ => cases h; simp [eval]
+    | add _ _ _ _ =>
+      cases h --why cant i aesop here already?
+      have : v1 = eval env a_1 := by aesop
+      have : v2 = eval env a_2 := by aesop
+      aesop
+    | sub _ _ _ _ =>
+      cases h
+      have : v1 = eval env a_1 := by aesop
+      have : v2 = eval env a_2 := by aesop
+      aesop
+    | mul _ _ _ _ =>
+      cases h
+      have : v1 = eval env a_1 := by aesop
+      have : v2 = eval env a_2 := by aesop
+      aesop
+    | div _ _ _ _ =>
+      cases h
+      have : v1 = eval env a_1 := by aesop
+      have : v2 = eval env a_2 := by aesop
+      aesop
+  · intro h
+    induction a generalizing i
+    all_goals
+      simp [h, eval]
+      aesop (add safe BigStep)
 
 /- 1.2 (1 point). Prove the following theorem to validate your definition
 above.
@@ -46,15 +83,15 @@ Hint: It may help to first prove
 `(AExp.add (AExp.num 2) (AExp.num 2), env) ⟹ 2 + 2`. -/
 
 theorem BigStep_add_two_two (env : Envir) :
-    (AExp.add (AExp.num 2) (AExp.num 2), env) ⟹ 4 :=
-  sorry
+    (AExp.add (AExp.num 2) (AExp.num 2), env) ⟹ 4 := by simp [eval]
+
 
 /- 1.3 (2 points). Prove that the big-step semantics is sound with respect to
 the `eval` function: -/
 
 theorem BigStep_sound (aenv : AExp × Envir) (i : ℤ) (hstep : aenv ⟹ i) :
-    eval (Prod.snd aenv) (Prod.fst aenv) = i :=
-  sorry
+    eval (Prod.snd aenv) (Prod.fst aenv) = i := by
+      simp [(bla (Prod.fst aenv) (Prod.snd aenv) i).mp hstep]
 
 
 /- ## Question 2 (5 points + 1 bonus point): Semantics of Regular Expressions
@@ -123,36 +160,68 @@ inductive Matches {α : Type} : Regex α → List α → Prop
 2.1 (1 point). Explain why there is no rule for `nothing`. -/
 
 -- enter your answer here
+--nothing is supposed to never match. In an inductive we only supply what *is* matched
 
 /- 2.2 (4 points). Prove the following inversion rules. -/
 
 @[simp] theorem Matches_atom {α : Type} {s : List α} {a : α} :
-    Matches (Regex.atom a) s ↔ s = [a] :=
-  sorry
+    Matches (Regex.atom a) s ↔ s = [a] := by
+      apply Iff.intro
+      · intro h
+        cases h
+        rfl
+      · aesop (add safe Matches)
+
+
 
 @[simp] theorem Matches_nothing {α : Type} {s : List α} :
-    ¬ Matches Regex.nothing s :=
-  sorry
+    ¬ Matches Regex.nothing s := by
+    intro h
+    cases h
+
 
 @[simp] theorem Matches_empty {α : Type} {s : List α} :
-    Matches Regex.empty s ↔ s = [] :=
-  sorry
+    Matches Regex.empty s ↔ s = [] := by
+      apply Iff.intro
+      · intro h
+        cases h
+        rfl
+      · aesop (add safe Matches)
 
 @[simp] theorem Matches_concat {α : Type} {s : List α} {r₁ r₂ : Regex α} :
     Matches (Regex.concat r₁ r₂) s
-    ↔ (∃s₁ s₂, Matches r₁ s₁ ∧ Matches r₂ s₂ ∧ s = s₁ ++ s₂) :=
-  sorry
+    ↔ (∃s₁ s₂, Matches r₁ s₁ ∧ Matches r₂ s₂ ∧ s = s₁ ++ s₂) := by
+    apply Iff.intro
+    intro h
+    cases h
+    · aesop
+    · intro h2
+      aesop (add safe Matches)
 
 @[simp] theorem Matches_alt {α : Type} {s : List α} {r₁ r₂ : Regex α} :
-    Matches (Regex.alt r₁ r₂) s ↔ (Matches r₁ s ∨ Matches r₂ s) :=
-  sorry
+    Matches (Regex.alt r₁ r₂) s ↔ (Matches r₁ s ∨ Matches r₂ s) := by
+      apply Iff.intro
+      · intro h
+        cases h
+        · aesop
+        · aesop
+      · intro h
+        cases h
+        · aesop (add unsafe Matches.alt_left, unsafe Matches.alt_right)
+        · aesop (add unsafe Matches.alt_left, unsafe Matches.alt_right)
 
 /- 2.3 (1 bonus point). Prove the following inversion rule. -/
 
 theorem Matches_star {α : Type} {s : List α} {r : Regex α} :
     Matches (Regex.star r) s ↔
     s = []
-    ∨ (∃s₁ s₂, Matches r s₁ ∧ Matches (Regex.star r) s₂ ∧ s = s₁ ++ s₂) :=
-  sorry
+    ∨ (∃s₁ s₂, Matches r s₁ ∧ Matches (Regex.star r) s₂ ∧ s = s₁ ++ s₂) := by
+      apply Iff.intro
+      · intro h
+        cases h
+        all_goals aesop
+      · intro h
+        cases h
+        all_goals aesop (add unsafe Matches)
 
 end LoVe
